needs only adequate documentation

theories/NormalIsomorphism.v
@@ -34,3 +34,94 @@ Proof.
     fold (θ' (App s (θ (ψ t))) l).
     now rewrite H0.
 Qed.
+
+(*        Digression:      *)
+(* proof using isomorphism *)
+(* ----------------------- *)
+
+Definition irreducible s := ~exists t, Lambda.step s t.
+
+Theorem nfs_are_irreducible :
+  (forall s, Lambda.normal s -> irreducible s)
+  /\
+  (forall s, apps s -> irreducible s).
+Proof.
+  apply Lambda.mut_normal_ind ; intros.
+  - intro.
+    apply H.
+    destruct H0 as [t Ht].
+    inversion Ht.
+    now exists s'.
+    - intro.
+      apply H.
+      destruct H0 as [t Ht].
+      now exists t.
+    - intro.
+      now destruct H.
+    - intro.
+      destruct H1 as [t0 Ht0].
+      inversion Ht0 ; subst.
+      + inversion a.
+      + apply H. now exists s'.
+      + apply H0. now exists t'.
+Qed.
+
+Theorem irreducible_is_nf s :
+  irreducible s -> Lambda.normal s.
+Proof.
+  induction s ; intro H.
+  - constructor. constructor.
+  - constructor. apply IHs.
+    intro. apply H.
+    inversion H0.
+    apply Step_Abs in H1.
+    now exists (Lam x).
+  - constructor. constructor.
+    + assert (Hs1 : irreducible s1).
+      { intro. apply H.
+        inversion H0.
+        eapply Step_App1 in H1. eauto. }
+      apply IHs1 in Hs1. inversion Hs1.
+      * cut False ; [contradiction |].
+        subst. apply H.
+        exists (s.[s2/]). now constructor.
+      * assumption.
+    + apply IHs2. intro. apply H.
+      inversion H0.
+      apply Step_App2 with (s:=s1) in H1. 
+      now exists (App s1 x).
+Qed.
+
+Definition irreducible' t := ~exists t', Canonical.step t t'.
+
+Conjecture nts_are_irreducible :
+  forall t, Canonical.normal t -> irreducible' t.
+
+Conjecture irreducible_is_nt :
+  forall t, irreducible' t -> Canonical.normal t.
+
+Corollary nf_inclusion s :
+  Lambda.normal s -> Canonical.normal (ψ s).
+Proof.
+  intro H.
+  apply nfs_are_irreducible in H.
+  cut (irreducible' (ψ s)).
+  - apply irreducible_is_nt.
+  - intro. apply H.
+    inversion H0. apply θ_step_pres in H1.
+    rewrite LambdaIsomorphism.inversion2 in H1.
+    now exists (θ x).
+Qed.
+
+Corollary nt_inclusion t :
+  Canonical.normal t -> Lambda.normal (θ t).
+Proof.
+  intro H.
+  apply nts_are_irreducible in H.
+  cut (irreducible (θ t)).
+  - apply irreducible_is_nf.
+  - intro. apply H.
+    inversion H0. apply ψ_step_pres in H1.
+    rewrite (proj1 LambdaIsomorphism.inversion1) in H1.
+    now exists (ψ x).
+Qed.
